

$$3.2. A = \{1, 2\}, B = \{a, b, c\}.$$

$$B^A = \{f_1, f_2, \dots, f_9\}$$

$$f_1 = \{\langle 1, a \rangle, \langle 2, a \rangle\}, f_2 = \{\langle 1, a \rangle, \langle 2, b \rangle\}, f_3 = \{\langle 1, a \rangle, \langle 2, c \rangle\}$$

$$f_4 = \{\langle 1, b \rangle, \langle 2, a \rangle\}, f_5 = \{\langle 1, b \rangle, \langle 2, b \rangle\}, f_6 = \{\langle 1, b \rangle, \langle 2, c \rangle\}$$

$$f_7 = \{\langle 1, c \rangle, \langle 2, a \rangle\}, f_8 = \{\langle 1, c \rangle, \langle 2, b \rangle\}, f_9 = \{\langle 1, c \rangle, \langle 2, c \rangle\}$$

$$3.5. (1) \checkmark (2) \times (3) \times (4) \times$$

$$3.14. X_A = \{\langle a, 1 \rangle, \langle b, 1 \rangle, \langle c, 0 \rangle, \langle d, 0 \rangle\}$$

$$X_B = \{\langle a, 0 \rangle, \langle b, 1 \rangle, \langle c, 0 \rangle, \langle d, 1 \rangle\}$$

$$X_{A \cap B} = \{\langle a, 0 \rangle, \langle b, 1 \rangle, \langle c, 0 \rangle, \langle d, 0 \rangle\}$$

$$3.19. (1) g \circ f = (x+y)^2 - 2 = x^2 + 8x + 14.$$

$$f \circ g = x^2 - 2 + y = x^2 + 2$$

(2). 都不是单射. 都不是满射, 都不是双射.

$$(3). \textcircled{g}^{-1} = x - y.$$

$$h^{-1} = \sqrt[3]{x+1}$$

$$3.30. \text{ 令 } f: [1, 2] \rightarrow [0, 1].$$

$$f(x) = x - 1.$$

则  $f$  为从  $[1, 2]$  到  $[0, 1]$  的双射函数.

3.38.

(1).  $\mathbb{Z}$ . (2).  $\mathbb{N}_0$  (3)  $\mathbb{N}_0$  (4)  $\mathbb{N}_0$  (5)  $\mathbb{N}_0$  (6)  $\mathbb{N}$ .